driver/Compiler.v
@@ -224,7 +224,7 @@ Definition transf_c_program_bytes (p: Csyntax.program) : res (list Integers.byte
   @@@ time "Generation of the symbol table" Symbtablegen.transf_program
   (* @@@ time "Normalize the symbol table indexes" NormalizeSymb.transf_program *)
   @@@ time "Generation of relocation table" Reloctablesgen.transf_program
-  @@@ time "Encoding of instructions and data" RelocBingen.transf_program
+  @@@ time "Encoding of instructions and data" (RelocBingen.transf_program true)
   (* @@@ time "Added the starting stub code" Stubgen.transf_program *)
   @@ time "Removing addendums" RemoveAddend.transf_program
   @@@ time "Encoding of tables" TablesEncode.transf_program
@@ -240,7 +240,7 @@ Definition transf_c_program_bytes_more (p: Csyntax.program) : res (list Integers
   @@@ time "Generation of the symbol table" Symbtablegen.transf_program
   (* @@@ time "Normalize the symbol table indexes" NormalizeSymb.transf_program *)
   @@@ time "Generation of relocation table" Reloctablesgen2.transf_program
-  @@@ time "Encoding of instructions and data" RelocBingen.transf_program
+  @@@ time "Encoding of instructions and data" (RelocBingen.transf_program true)
   (* @@@ time "Added the starting stub code" Stubgen.transf_program *)
   @@ time "Removing addendums" RemoveAddend.transf_program
   @@@ time "Encoding of tables" TablesEncode.transf_program
@@ -254,7 +254,7 @@ Definition transf_c_program_bytes' (p: Csyntax.program) :=
   @@ time "Pad space to make the alignment of data correct" PadInitData.transf_program
   @@@ time "Generation of the symbol table" Symbtablegen.transf_program
   @@@ time "Generation of relocation table" Reloctablesgen.transf_program
-  @@@ time "Encoding of instructions and data" RelocBingen.transf_program
+  @@@ time "Encoding of instructions and data" (RelocBingen.transf_program true)
   @@ time "Removing addendums" RemoveAddend.transf_program
   @@@ time "Encoding of tables" TablesEncode.transf_program
   @@@ time "Generation of the reloctable Elf" RelocElfgen.gen_reloc_elf
@@ -561,7 +561,7 @@ Proof.
   destruct (Asmlabelgen.transf_program p1) eqn:RTP; simpl in T; try discriminate.
   destruct (Symbtablegen.transf_program (PadInitData.transf_program (PadNops.transf_program p0))) eqn:STG; simpl in T; try discriminate.
   destruct (Reloctablesgen.transf_program p2) eqn: RTG; simpl in T; try discriminate.
-  destruct (RelocBingen.transf_program p3) eqn: RBG; simpl in T; try discriminate.
+  destruct (RelocBingen.transf_program true p3) eqn: RBG; simpl in T; try discriminate.
   destruct (TablesEncode.transf_program (RemoveAddend.transf_program p4)) eqn: TE; simpl in T; try discriminate.
   destruct (RelocElfgen.gen_reloc_elf p5) eqn:GRE; simpl in T; try discriminate.
   red.
